Constraint System work

Clap/eDSLState/ConstraintSystem/fpMul.lean
@@ -1,4 +1,5 @@
 import Clap.eDSLState.HashCons.Eval
+import Clap.eDSLState.ConstraintSystem.isZero
 import Clap.eDSLState.ConstraintSystem.num2bits
 
 namespace Clap
@@ -9,10 +10,11 @@ section Bob
 
 open HashConsM
 
-def rangeCheckVec {p k : ℕ} (numAlloc width : ℕ) (vec : Vector (BoundRef p) k) : HashConsM p (Array (BoundRef p) × ℕ) := do
-  vec.foldlM (b := (#[], numAlloc)) fun (acc, numAlloc) elem ↦ do
-    let (cs, numAlloc) ← num2bits width numAlloc elem
-    return (acc ++ cs, numAlloc)
+--k*width+k constraints, k*width allocations
+def rangeCheckVec {p k : ℕ} (constraints : Array (BoundRef p)) (numAlloc width : ℕ) (vec : Vector (BoundRef p) k) : HashConsM p (Array (BoundRef p) × ℕ) := do
+  vec.foldlM (b := (constraints, numAlloc)) fun (constraints, numAlloc) elem ↦ do
+    let (_bits, constraints, numAlloc) ← num2bits constraints numAlloc width elem
+    return (constraints, numAlloc)
 
 def evalPoly {p k : ℕ} (coeffs : Vector (BoundRef p) k) (x : ZMod p) : HashConsM p (BoundRef p) := do
   (List.finRange k).foldrM
@@ -21,6 +23,7 @@ def evalPoly {p k : ℕ} (coeffs : Vector (BoundRef p) k) (x : ZMod p) : HashCon
       acc + term
     ) (←mkConstant 0)
 
+-- return size 2*k - 1
 def assertPolyEqProd {p k : ℕ}
     (a : Vector (BoundRef p) k)
     (b : Vector (BoundRef p) k)
@@ -30,17 +33,19 @@ def assertPolyEqProd {p k : ℕ}
       let mul ← (←evalPoly a k) * (←evalPoly b k)
       mul - (←evalPoly c k)
 
+-- 3*k*width + 3*k constraints, 3*k*width allocations
 def rangeCheckInputs
   {p k : ℕ}
   (constraints : Array (BoundRef p)) (numAlloc : ℕ)
   (width : ℕ)
   (a b p' : Vector (BoundRef p) k)
 : HashConsM p (Array (BoundRef p) × ℕ) := do
-  let (constraints₁, numAlloc) ← rangeCheckVec numAlloc width a
-  let (constraints₂, numAlloc) ← rangeCheckVec numAlloc width b
-  let (constraints₃, numAlloc) ← rangeCheckVec numAlloc width p'
-  return (constraints ++ constraints₁ ++ constraints₂ ++ constraints₃, numAlloc)
+  let (constraints, numAlloc) ← rangeCheckVec constraints numAlloc width a
+  let (constraints, numAlloc) ← rangeCheckVec constraints numAlloc width b
+  let (constraints, numAlloc) ← rangeCheckVec constraints numAlloc width p'
+  return (constraints, numAlloc)
 
+-- k allocations
 def allocUnchecked
   {p : ℕ}
   (numAlloc : ℕ)
@@ -49,6 +54,7 @@ def allocUnchecked
   let vec ← Vector.ofFnM fun i : Fin k ↦ mkVar (numAlloc + i)
   return (vec, numAlloc + k)
 
+--k*width+k constraints, k*width+k allocations
 def allocRangeChecked
   {p : ℕ}
   (constraints : Array (BoundRef p)) (numAlloc : ℕ)
@@ -56,9 +62,10 @@ def allocRangeChecked
   (width : ℕ)
 : HashConsM p (Vector (BoundRef p) k × (Array (BoundRef p) × ℕ)) := do
   let (vec, numAlloc) ← allocUnchecked numAlloc k
-  let (range_check_constraints, numAlloc) ← rangeCheckVec numAlloc width vec
-  return (vec, (constraints ++ range_check_constraints, numAlloc))
+  let (constraints, numAlloc) ← rangeCheckVec constraints numAlloc width vec
+  return (vec, (constraints, numAlloc))
 
+-- 2*k-1 constraints, k allocations
 def polyMult
   {p k : ℕ}
   (constraints : Array (BoundRef p)) (numAlloc : ℕ)
@@ -68,6 +75,13 @@ def polyMult
   let prodConstraints ← assertPolyEqProd a b ab
   return (ab, (constraints ++ prodConstraints, numAlloc))
 
+-- if k = 0 then 0 allocations, 0 constraints
+-- else k-1 allocations
+--      0 constraints
+/-
+        + (k-1) * 1 + num2bits.num_constraints (width + Nat.clog 2 k + 2)
+        + 1
+-/
 def check_carry_zero
   {p : ℕ}
   {k : ℕ}
@@ -83,11 +97,11 @@ def check_carry_zero
         then pure t[i]
         else t[i] + carry[(⟨i - 1, by omega⟩ : Fin (k - 1))]
       let constraints := constraints.push (←e - (←(←mkConstant (2^width)) * carry[i]))
-      let (num2bits_constraints, numAlloc) ← num2bits
+      let (_bits, constraints, numAlloc) ← num2bits
           (width := width + Nat.clog 2 k + 2)
-          (numAlloc := numAlloc)
+          (numAlloc := numAlloc) (constraints := constraints)
           (expr := ← carry[i] + (←mkConstant (k * 2 ^ (width + 1))))
-      return (constraints ++ num2bits_constraints, numAlloc)
+      return (constraints, numAlloc)
     ) (constraints, numAlloc)
     let overflow ← t[(⟨k - 1, by omega⟩ : Fin k)] + (
         ←if _ : k = 1 then mkConstant 0
@@ -95,6 +109,21 @@ def check_carry_zero
     )
     return (constraints.push overflow, numAlloc)
 
+def mkOr {p} (a b : BoundRef p) : HashConsM p (BoundRef p) := do
+  (←a + b) - (←a*b)
+
+def mkNot {p} (a : BoundRef p) : HashConsM p (BoundRef p) := do
+  (←mkConstant 1) - a
+
+/-
+k = 0 : 1 constraints, 0 allocations
+k = n+1 :
+  num2bits : width+1 constraints, width allocations
+  isZero : 2 constraints, 2 allocations
+
+constraints : 1 + k*(width + 3)
+allocations : k*(width + 2)
+-/
 def check_lt_impl
   {p : ℕ}
   {k : ℕ}
@@ -106,19 +135,26 @@ def check_lt_impl
   match _ : k with
   | .zero => return (constraints.push (←isLt - (←mkConstant 1)), numAlloc)
   | .succ k =>
-    let (constraints, numAlloc) ← num2bits
+    let (_bits, constraints, numAlloc) ← num2bits
+      (constraints := constraints)
       (numAlloc := numAlloc)
       (width := width)
       (expr := ←
-        (←(←mkConstant 1) - isLt) * 
+        (←(←mkConstant 1) - isLt) *
         (←
           (←a[Fin.last k] - b[Fin.last k]) +
           (←mkConstant ((2 ^ width : ZMod p) - 1))
         )
       )
 
-    let x ← mkConstant 0
-    return (constraints, numAlloc)
+    let (isz, constraints, numAlloc) ← isZero constraints numAlloc (←a[Fin.last k] - b[Fin.last k])
+
+    let isLt' ← mkOr isLt (←mkNot isz)
+
+    let a' := Vector.ofFn (fun (i : Fin k) ↦ a[i.castSucc])
+    let b' := Vector.ofFn (fun (i : Fin k) ↦ b[i.castSucc])
+
+    check_lt_impl constraints numAlloc width isLt' a' b'
 
 def check_lt
   {p : ℕ}
@@ -129,7 +165,29 @@ def check_lt
 : HashConsM p (Array (BoundRef p) × ℕ) := do
   check_lt_impl constraints numAlloc width (←mkConstant 0) a b
 
-def fpMul {p : ℕ} (width k numAlloc : ℕ) (a b p' : Vector (BoundRef p) k) : HashConsM p (Array (BoundRef p) × ℕ) := do
+def inner
+  {p}
+  {k}
+  (constraints : Array (BoundRef p))
+  (ab t : Vector (BoundRef p) (2*k-1))
+  (p' q r : Vector (BoundRef p) k)
+:
+  HashConsM p (Array (BoundRef p))
+:= do
+  (List.range (2*k - 1)).foldrM (λ (x : ℕ) constraints ↦ do
+    let pq_plus_r ← (←(←evalPoly p' x) * (←evalPoly q x)) + (←evalPoly r x)
+    let ab_sub ← (←evalPoly ab x) - pq_plus_r
+    let res ← (←evalPoly t x) - ab_sub
+    return constraints.push res
+  ) (constraints)
+
+def fpMul_impl {p : ℕ}
+  (numAlloc : ℕ)
+  (width k : ℕ)
+  (a b p' : Vector (BoundRef p) k)
+:
+  HashConsM p (Vector (BoundRef p) k × Array (BoundRef p) × ℕ)
+:= do
   let (constraints, numAlloc) ← rangeCheckInputs #[] numAlloc width a b p'
 
   let (ab, (constraints, numAlloc)) ← polyMult constraints numAlloc a b
@@ -138,16 +196,393 @@ def fpMul {p : ℕ} (width k numAlloc : ℕ) (a b p' : Vector (BoundRef p) k) : 
   let (r, (constraints, numAlloc)) ← allocRangeChecked constraints numAlloc k width
   let (t, numAlloc) ← allocUnchecked numAlloc (2*k - 1)
 
-  let constraints ← (List.range (2*k - 1)).foldrM (λ (x : ℕ) constraints ↦ do
-    let pq_plus_r ← (←(←evalPoly p' x) * (←evalPoly q x)) + (←evalPoly r x)
-    let ab_sub ← (←evalPoly ab x) - pq_plus_r
-    let res ← (←evalPoly t x) - ab_sub
-    return constraints.push res
-  ) (constraints)
+  let constraints ← inner constraints ab t p' q r
 
   let (constraints, numAlloc) ← check_carry_zero constraints numAlloc width t
 
-  check_lt constraints numAlloc width r p'
+  let (constraints, numAlloc) ← check_lt constraints numAlloc width r p'
+
+  return (r, constraints, numAlloc)
+
+def fpMul {p : ℕ}
+  (constraints : Array ExprRef) (numAlloc : ℕ)
+  (width k : ℕ)
+  (a b p' : Vector (BoundRef p) k)
+:
+  HashConsM p (Vector (BoundRef p) k × Array (BoundRef p) × ℕ)
+:= do
+  let (result, fpmul_constraints, numAlloc) ← fpMul_impl
+    (numAlloc := numAlloc)
+    (width := width)
+    (k := k)
+    a b p'
+  return (result, constraints ++ fpmul_constraints, numAlloc)
+
+
+namespace fpMul
+
+def num_constraints (width k: ℕ) : ℕ :=
+  if k = 0 then 1
+  else
+    -- TODO fix priority on deref
+    (Nat.mul 2 (k-1)) * (Nat.clog 2 (2 * k - 1) : ℕ) +
+    (8*k-2) * width +
+    20*k
+    - 8
+
+
+def numAllocStep (width k : ℕ) : ℕ := if k = 0 then 0
+else
+  (k * 6) * num2bits.numAllocStep width +
+  (8 * k - 4) +
+  (2 * k - 2) * num2bits.numAllocStep (width + Nat.clog 2 (2 * k - 1) + 2) +
+  k * isZero.numAllocStep
+
+@[simp, grind =]
+lemma allocUnchecked_numAllocStep
+  {p}
+  {numAlloc}
+  {k}
+  {σ : HashConsSt p}
+:
+  ((allocUnchecked numAlloc k).getResult σ).2 =
+  numAlloc + k
+:= by
+  simp [allocUnchecked]
+
+@[simp, grind =]
+lemma check_carry_zero_num_constraints
+  {p : ℕ}
+  {k}
+  {constraints : Array (BoundRef p)} {numAlloc : ℕ}
+  {width : ℕ}
+  {a : Vector (BoundRef p) k}
+  {σ}
+:
+  ((check_carry_zero constraints numAlloc width a).getResult σ).1.size =
+  constraints.size + if k = 0 then 0 else
+  (k-1) * (1 + num2bits.num_constraints (width + Nat.clog 2 k + 2)) + 1
+:= by
+  simp [check_carry_zero]
+  obtain _ | k := k
+  . simp
+  . obtain _ | k := k
+    . simp
+    . simp
+      set f := λ i x => _
+
+      have h_f (x) (constraints) (numAlloc) (σ) :
+        ((f x (constraints, numAlloc)).getResult σ).1.size =
+        constraints.size + 1 + num2bits.num_constraints (width + Nat.clog 2 (k + 1 + 1) + 2)
+      := by
+        subst f
+        simp
+        split <;> simp
+
+      generalize (allocUnchecked numAlloc (k + 1)).getHashConsState σ = σ
+      generalize numAlloc + (k + 1) = numAlloc
+      have : (List.finRange (k + 1)).length = k + 1 := by grind
+      set l := List.finRange (k + 1)
+      clear_value l
+      clear_value f
+      set x := width + Nat.clog 2 (k + 1 + 1) + 2
+      clear_value x
+      have :
+        (k + 1) * (1 + num2bits.num_constraints x) =
+        l.length * (1 + num2bits.num_constraints x)
+      := by grind
+      rewrite [this]
+      clear this
+      obtain _ | ⟨hd, tl⟩ := l
+      . exfalso; grind
+      . clear this
+        induction' tl with head tail h_tail
+        . simp [h_f, add_assoc]
+        . simp [h_f]
+          simp [h_f] at h_tail
+          rewrite [h_tail]
+          grind
+
+@[simp, grind =]
+lemma check_carry_zero_numAlloc
+  {p : ℕ}
+  {k}
+  {constraints : Array (BoundRef p)} {numAlloc : ℕ}
+  {width : ℕ}
+  {a : Vector (BoundRef p) k}
+  {σ}
+:
+  ((check_carry_zero constraints numAlloc width a).getResult σ).2 =
+  numAlloc + if k = 0
+  then 0
+  else ((k-1) * (1 + num2bits.numAllocStep (width + Nat.clog 2 k + 2)))
+:= by
+  simp [check_carry_zero]
+  obtain _ | k := k
+  . simp
+  . obtain _ | k := k
+    . simp
+    . simp
+      set f := λ i x => _
+
+      have h_f (x) (constraints) (numAlloc) (σ) :
+        ((f x (constraints, numAlloc)).getResult σ).2 =
+        numAlloc + num2bits.numAllocStep (width + Nat.clog 2 (k + 1 + 1) + 2)
+      := by
+        subst f
+        simp
+        split <;> simp
+
+      generalize (allocUnchecked numAlloc (k + 1)).getHashConsState σ = σ
+      have : (List.finRange (k + 1)).length = k + 1 := by grind
+      set l := List.finRange (k + 1)
+      clear_value l
+      clear_value f
+      set x := width + Nat.clog 2 (k + 1 + 1) + 2
+      clear_value x
+      have :
+        (k + 1) * (1 + num2bits.numAllocStep x) =
+        l.length * (1 + num2bits.numAllocStep x)
+      := by grind
+
+      rewrite [this]; clear this
+      rewrite [show numAlloc + (k + 1) = numAlloc + l.length by grind]
+      clear this
+      generalize eq:numAlloc + l.length = numAlloc'
+      rewrite [mul_add, mul_one, ←add_assoc, eq]
+      clear eq
+      induction' l with head tail ih generalizing numAlloc'
+      . grind
+      . simp [h_f]
+        rewrite [ih]
+        grind
+
+@[simp, grind =]
+lemma check_lt_num_constraints
+  {p : ℕ}
+  {k}
+  {constraints : Array (BoundRef p)} {numAlloc : ℕ}
+  {width : ℕ}
+  {a b : Vector (BoundRef p) k}
+  {σ}
+:
+  ((check_lt constraints numAlloc width a b).getResult σ).1.size =
+  constraints.size + 1 + k*(width + 3)
+:= by
+  simp [check_lt]
+  generalize ((mkConstant 0).getResult σ) = isLt
+  generalize ((mkConstant 0).getHashConsState σ) = σ
+  induction' k with k h_k generalizing isLt σ constraints numAlloc width
+  . simp [check_lt_impl]
+  . unfold check_lt_impl
+    set a' := Vector.ofFn (λ i => a[i.castSucc])
+    set b' := Vector.ofFn (λ i => b[i.castSucc])
+    simp [getResult_bind]
+    rewrite [h_k]
+    simp [num2bits.num_constraints, isZero.num_constraints]
+    grind
+
+@[simp, grind =]
+lemma check_lt_numAlloc
+  {p : ℕ}
+  {k}
+  {constraints : Array (BoundRef p)} {numAlloc : ℕ}
+  {width : ℕ}
+  {a b : Vector (BoundRef p) k}
+  {σ}
+:
+  ((check_lt constraints numAlloc width a b).getResult σ).2 =
+  numAlloc + k*(num2bits.numAllocStep width + isZero.numAllocStep)
+:= by
+  simp [check_lt]
+  generalize ((mkConstant 0).getResult σ) = isLt
+  generalize ((mkConstant 0).getHashConsState σ) = σ
+  induction' k with k h_k generalizing isLt σ constraints numAlloc width
+  . simp [check_lt_impl]
+  . unfold check_lt_impl
+    set a' := Vector.ofFn (λ i => a[i.castSucc])
+    set b' := Vector.ofFn (λ i => b[i.castSucc])
+    simp [getResult_bind]
+    rewrite [h_k]
+    grind
+
+@[simp, grind =]
+lemma inner_num_constraints
+  {p}
+  {k}
+  {constraints : Array (BoundRef p)}
+  {ab t : Vector (BoundRef p) (2*k-1)}
+  {p' q r}
+  {σ}
+:
+  ((inner constraints ab t p' q r).getResult σ).size =
+  constraints.size + (2*k-1)
+:= by
+  unfold inner
+  simp [←bind_assoc, -bind_pure_comp]
+
+  have (length) (f : ℕ → HashConsM p (BoundRef p)) :
+    (((List.range length).foldrM (λ x (constraints : Array (BoundRef p)) => do
+      let x ← f x
+      pure (constraints.push x)
+    ) constraints).getResult σ).size = constraints.size + length
+  := by
+    induction length
+    . simp
+    . simp
+
+  rw [this]
+
+@[simp, grind =]
+lemma rangeCheckVec_num_constraints
+  {p}
+  {k width}
+  {constraints : Array (BoundRef p)}
+  {numAlloc : ℕ}
+  {vec : Vector (BoundRef p) k}
+  {σ}
+:
+  ((rangeCheckVec constraints numAlloc width vec).getResult σ).1.size =
+  constraints.size + k*(width + 1)
+:= by
+  unfold rangeCheckVec
+  obtain ⟨⟨l⟩, h_l⟩ := vec
+  induction' l with x l ih generalizing k constraints numAlloc σ
+  . simp
+    grind
+  . obtain _ | k := k
+    . exfalso; grind
+    simp at ⊢ ih
+    rewrite [ih (k := k)]
+    . simp [num2bits.num_constraints]
+      grind
+    . grind
+
+@[simp, grind =]
+lemma rangeCheckVec_numAlloc
+  {p}
+  {k width : ℕ}
+  {constraints : Array (BoundRef p)}
+  {numAlloc : ℕ}
+  {vec : Vector (BoundRef p) k}
+  {σ}
+:
+  ((rangeCheckVec constraints numAlloc width vec).getResult σ).2 =
+  numAlloc + k * (num2bits.numAllocStep width)
+:= by
+  unfold rangeCheckVec
+  obtain ⟨⟨l⟩, h_l⟩ := vec
+  induction' l with x l ih generalizing k constraints numAlloc σ
+  . simp [←h_l]
+  . obtain _ | k := k
+    . exfalso; grind
+    simp at ⊢ ih
+    rewrite [ih (k := k)]
+    . simp
+      grind
+    . grind
+
+@[simp, grind =]
+lemma allocRangeChecked_num_constraints
+  {p}
+  {k width}
+  {constraints : Array (BoundRef p)}
+  {numAlloc : ℕ}
+  {σ}
+:
+  ((allocRangeChecked constraints numAlloc k width).getResult σ).2.1.size =
+  constraints.size + k*(width + 1)
+:= by
+  unfold allocRangeChecked
+  simp
+
+@[simp, grind =]
+lemma allocRangeChecked_numAlloc
+  {p}
+  {k width}
+  {constraints : Array (BoundRef p)}
+  {numAlloc : ℕ}
+  {σ}
+:
+  ((allocRangeChecked constraints numAlloc k width).getResult σ).2.2 =
+  numAlloc + k * (1 + num2bits.numAllocStep width)
+:= by
+  unfold allocRangeChecked
+  simp
+  grind
+
+@[simp, grind =]
+lemma polyMult_num_constraints
+  {p}
+  {k}
+  {constraints : Array (BoundRef p)}
+  {numAlloc}
+  {a b : Vector (BoundRef p) k}
+  {σ : HashConsSt p}
+:
+  ((polyMult constraints numAlloc a b).getResult σ).2.1.size =
+  constraints.size + (2*k-1)
+:= by
+  unfold polyMult assertPolyEqProd
+  simp
+
+@[simp, grind =]
+lemma polyMult_numAlloc
+  {p}
+  {k}
+  {constraints : Array (BoundRef p)}
+  {numAlloc}
+  {a b : Vector (BoundRef p) k}
+  {σ : HashConsSt p}
+:
+  ((polyMult constraints numAlloc a b).getResult σ).2.2 =
+  numAlloc + (2*k-1)
+:= by
+  unfold polyMult assertPolyEqProd
+  simp
+
+@[simp, grind =]
+lemma num_constraints_eq
+  {p : ℕ}
+  {constraints} {numAlloc}
+  {width k}
+  {a b p'}
+  {σ : HashConsSt p}
+:
+  ((fpMul constraints numAlloc width k a b p').getResult σ).2.1.size =
+  constraints.size + num_constraints width k
+:= by
+  simp [
+    fpMul,
+    fpMul_impl,
+    rangeCheckInputs,
+    num2bits.num_constraints
+  ]
+  obtain _ | k := k
+  . simp [num_constraints]
+  . rewrite [ite_cond_eq_false]
+    . grind [num_constraints]
+    . grind
+
+
+
+
+@[simp, grind =]
+lemma numAllocStep_eq
+  {p : ℕ}
+  {constraints} {numAlloc}
+  {width k}
+  {a b p'}
+  {σ : HashConsSt p}
+:
+  ((fpMul constraints numAlloc width k a b p').getResult σ).2.2 =
+  numAlloc + numAllocStep width k
+:= by
+  simp [fpMul, fpMul_impl, numAllocStep, rangeCheckInputs]
+  grind
+
+end fpMul
+
 
 end Bob
 
