Clap/eDSLState/ConstraintSystem/num2bits.lean
@@ -12,12 +12,60 @@ def mkBits2num {p : ℕ} (bits : Array ExprRef) : HashConsM p ExprRef := do
   let init ← mkConstant 0
   bits.foldrM (λ bit acc => do mkAdd bit (←mkMul (←mkConstant 2) acc)) init
 
-def num2bits {p : ℕ} (width numAlloc : ℕ) (expr : ExprRef) : HashConsM p (Array ExprRef × ℕ) := do
+def num2bits_impl {p : ℕ}
+  (numAlloc : ℕ)
+  (width : ℕ) (expr : ExprRef)
+:
+  HashConsM p (Array (BoundRef p) × Array ExprRef × ℕ)
+:= do
   let bits ← (Array.range width).mapM (λ idx => mkVar (numAlloc + idx))
   let bit_constraints ← bits.mapM (λ bit => do mkMul bit (←mkSub (←mkConstant 1) bit)) -- equivalent to assert_bit_e
   let value_constraint ← mkSub (←mkBits2num bits) expr
   let constraints := bit_constraints.push value_constraint
-  return (constraints, numAlloc + width)
+  return (bits, constraints, numAlloc + width)
+
+def num2bits {p : ℕ}
+  (constraints : Array (BoundRef p) )(numAlloc : ℕ)
+  (width : ℕ) (expr : ExprRef)
+:
+  HashConsM p (Array (BoundRef p) × Array ExprRef × ℕ)
+:= do
+  let (bits, num2bits_constraints, numAlloc) ← num2bits_impl numAlloc width expr
+  return (bits, constraints ++ num2bits_constraints, numAlloc)
+
+namespace num2bits
+
+def num_constraints (width : ℕ) : ℕ := width + 1
+def numAllocStep (width : ℕ) : ℕ := width
+
+@[simp, grind =]
+lemma num_constraints_eq
+  {p : ℕ}
+  {constraints} {numAlloc}
+  {width}
+  {expr}
+  {σ : HashConsSt p}
+:
+  ((num2bits constraints numAlloc width expr).getResult σ).2.1.size =
+  constraints.size + num_constraints width
+:= by
+  simp [num2bits, num2bits_impl, num_constraints]
+
+@[simp, grind =]
+lemma numAllocStep_eq
+  {p : ℕ}
+  {constraints} {numAlloc}
+  {width}
+  {expr}
+  {σ : HashConsSt p}
+:
+  ((num2bits constraints numAlloc width expr).getResult σ).2.2 =
+  numAlloc + numAllocStep width
+:= by
+  simp [num2bits, num2bits_impl, numAllocStep]
+
+end num2bits
+
 
 end Bob
 
