Clap/eDSLState/ConstraintSystem/isZero.lean
@@ -1,0 +1,49 @@
+import Clap.eDSLState.HashCons.Eval
+
+namespace Clap.ConstraintSystem
+
+open HashConsM
+
+def isZero {p}
+  (constraints : Array ExprRef) (numAlloc : ℕ)
+  (expr : ExprRef)
+:
+  HashConsM p (ExprRef × Array ExprRef × ℕ)
+:= do
+  let inv ← mkVar numAlloc
+  let o ← mkVar (numAlloc + 1)
+  let constraint1 ← (←((←mkConstant 1) - (←inv * expr))) - o
+  let constraint2 ← o * expr
+  return (o, constraints.append #[constraint1, constraint2], numAlloc + 2)
+
+namespace isZero
+
+def num_constraints : ℕ := 2
+def numAllocStep : ℕ := 2
+
+@[simp, grind =]
+lemma num_constraints_eq
+  {p : ℕ}
+  {constraints} {numAlloc}
+  {expr}
+  {σ : HashConsSt p}
+:
+  ((isZero constraints numAlloc expr).getResult σ).2.1.size =
+  constraints.size + num_constraints
+:= by
+  simp [isZero, num_constraints]
+
+@[simp, grind =]
+lemma numAllocStep_eq
+  {p : ℕ}
+  {constraints} {numAlloc}
+  {expr}
+  {σ : HashConsSt p}
+:
+  ((isZero constraints numAlloc expr).getResult σ).2.2 =
+  numAlloc + numAllocStep
+:= by
+  simp [isZero, numAllocStep]
+
+end isZero
+end Clap.ConstraintSystem
