Clap/eDSLState/ConstraintSystem/share.lean
@@ -1,0 +1,56 @@
+import Clap.eDSLState.HashCons.Eval
+
+namespace Clap
+
+namespace ConstraintSystem
+
+section Bob
+
+open HashConsM
+
+def share {p : ℕ}
+  (constraints : Array (BoundRef p)) (numAlloc : ℕ)
+  (expr : BoundRef p)
+:
+  HashConsM p (BoundRef p × Array (BoundRef p) × ℕ)
+:= do
+  let v ← mkVar numAlloc
+  let s ← expr - v
+  return (v, constraints.push s, numAlloc + 1)
+
+namespace share
+
+def num_constraints : ℕ := 1
+def numAllocStep : ℕ := 1
+
+@[simp, grind =]
+lemma num_constraints_eq
+  {p : ℕ}
+  {constraints} {numAlloc}
+  {expr}
+  {σ : HashConsSt p}
+:
+  ((share constraints numAlloc expr).getResult σ).2.1.size =
+  constraints.size + num_constraints
+:= by
+  simp [share, num_constraints]
+
+@[simp, grind =]
+lemma numAllocStep_eq
+  {p : ℕ}
+  {constraints} {numAlloc}
+  {expr}
+  {σ : HashConsSt p}
+:
+  ((share constraints numAlloc expr).getResult σ).2.2 =
+  numAlloc + numAllocStep
+:= by
+  simp [share, numAllocStep]
+
+end share
+
+end Bob
+
+end ConstraintSystem
+
+end Clap
